src/protocol/DNS.Protocol.Parser.EverParseAdapter.fst
@@ -34,6 +34,10 @@ let generated_dns_uncompressed_question_srv_answer_packet_validator_linked : boo
 
 let generated_dns_uncompressed_question_txt_answer_packet_validator_linked : bool = true
 
+let generated_dns_opt_additional_packet_validator_linked : bool = true
+
+let generated_dns_uncompressed_question_opt_additional_packet_validator_linked : bool = true
+
 let generated_dns_header_validator = DNSProtocol.validate__dns_header
 
 let generated_dns_root_question_validator =
@@ -93,3 +97,12 @@ let generated_dns_uncompressed_question_txt_answer_packet_validator
     qname_length
     rr_name_length
     rdata_length
+
+let generated_dns_opt_additional_packet_validator option_payload_length =
+  DNSProtocol.validate__dns_opt_additional_packet option_payload_length
+
+let generated_dns_uncompressed_question_opt_additional_packet_validator
+    qname_length option_payload_length =
+  DNSProtocol.validate__dns_uncompressed_question_opt_additional_packet
+    qname_length
+    option_payload_length
